clean up insertion

formal-verification/FormalVerification/SemanticEquivalence/Insertion.lean
@@ -1,7 +1,4 @@
-import ProvenZk.Binary
-import ProvenZk.Hash
-import ProvenZk.Merkle
-import ProvenZk.Misc
+import ProvenZk
 
 import FormalVerification
 import FormalVerification.Utils
@@ -16,91 +13,7 @@ open SemaphoreMTB (F Order)
 open SemaphoreMTB renaming InsertionRound_30_30 → gInsertionRound
 open SemaphoreMTB renaming InsertionProof_4_30_4_4_30 → gInsertionProof
 
-lemma MerkleTree.item_at_nat_to_fin' {depth : Nat} {F: Type} {H: Hash F 2} (t : MerkleTree F H depth) (idx : Nat) (h : idx < 2 ^ depth):
-  MerkleTree.item_at_nat t idx = some (MerkleTree.tree_item_at_fin t ⟨idx, h⟩) := by
-  simp [MerkleTree.item_at_nat, MerkleTree.tree_item_at_fin]
-  simp [Dir.nat_to_dir_vec, Dir.fin_to_dir_vec]
-  simp [fin_to_bits_le_is_some h]
-  congr
-  apply Fin.eq_of_veq
-  apply Fin.val_cast_of_lt
-  assumption
 
-lemma nat_to_bits_le_some_when_lt :
-  nat_to_bits_le l a = some w → a < 2 ^ l := by
-  induction l generalizing a with
-  | zero =>
-    unfold nat_to_bits_le
-    split <;> simp [*]
-  | succ l ih =>
-    unfold nat_to_bits_le
-    simp [Bind.bind]
-    intro w h _
-    have := ih h
-    apply Nat.lt_of_div_lt_div (k := 2)
-    simpa [Nat.pow_succ]
-
-lemma MerkleTree.item_at_nat_some_when_le {D : Nat} {tree : MerkleTree α H D}:
-  MerkleTree.item_at_nat tree idx = some el → idx < 2 ^ D := by
-  intro h
-  unfold item_at_nat at h
-  unfold Dir.nat_to_dir_vec at h
-  simp at h
-  rcases h with ⟨a, h, -⟩
-  exact nat_to_bits_le_some_when_lt h
-
-lemma MerkleTree.item_at_nat_none_when_ge {D : Nat} {tree : MerkleTree α H D}:
-  idx ≥ 2^D → MerkleTree.item_at_nat tree idx = none := by
-  intro h
-  cases hp : item_at_nat tree idx
-  . rfl
-  . have := MerkleTree.item_at_nat_some_when_le hp
-    exfalso
-    exact not_lt_of_ge h this
-
-lemma MerkleTree.set_at_nat_some_when_le {D:Nat} {tree tree': MerkleTree α H D}:
-  MerkleTree.set_at_nat tree idx el = some tree' → idx < 2 ^ D := by
-  unfold MerkleTree.set_at_nat
-  unfold Dir.nat_to_dir_vec
-  simp
-  intro w h _
-  exact nat_to_bits_le_some_when_lt h
-
-
-lemma fin_to_bits_le_is_some' {depth : Nat} {idx : Nat} (h : idx < 2 ^ depth) :
-  nat_to_bits_le depth idx = some (fin_to_bits_le ⟨idx, h⟩) := by
-  simp [fin_to_bits_le]
-  split <;> tauto
-
-lemma MerkleTree.set_at_nat_to_fin' {depth : Nat} {F: Type} {H: Hash F 2} (t : MerkleTree F H depth) (idx : Nat) (item : F) (h : idx < 2 ^ depth):
-  MerkleTree.set_at_nat t idx item = some (MerkleTree.tree_set_at_fin t ⟨idx, h⟩ item) := by
-  simp [MerkleTree.set_at_nat, MerkleTree.tree_set_at_fin]
-  simp [Dir.nat_to_dir_vec]
-  simp [Dir.fin_to_dir_vec]
-  simp [fin_to_bits_le_is_some' h]
-
-lemma MerkleTree.set_at_nat_to_fin_some' {depth : Nat} {F: Type} {H: Hash F 2} {a : MerkleTree F H depth} (t : MerkleTree F H depth) (idx : Nat) (item : F) (h : idx < 2 ^ depth):
-  MerkleTree.set_at_nat t idx item = some a ↔
-  MerkleTree.tree_set_at_fin t ⟨idx, h⟩ item = a := by
-  rw [set_at_nat_to_fin' (h := h)]
-  simp
-
-lemma MerkleTree.item_at_nat_to_fin_some' {depth : Nat} {F: Type} {H: Hash F 2} {a : F} (t : MerkleTree F H depth) (idx : Nat) (h : idx < 2 ^ depth):
-  MerkleTree.item_at_nat t idx = some a ↔
-  MerkleTree.tree_item_at_fin t ⟨idx, h⟩ = a := by
-  rw [item_at_nat_to_fin' (h := h)]
-  . simp
-
-theorem MerkleTree.item_at_fin_invariant' {H : Hash α 2} {tree tree': MerkleTree α H depth} {ix₁ ix₂ : Fin (2 ^ depth)} { neq : ix₁ ≠ ix₂ }:
-  MerkleTree.tree_set_at_fin tree ix₁ item₁ = tree' →
-  MerkleTree.tree_item_at_fin tree' ix₂ = MerkleTree.tree_item_at_fin tree ix₂ := by
-  rw [<-set_at_nat_to_fin_some' (h := ix₁.2)]
-  rw [<-item_at_nat_to_fin_some' (h := ix₂.2)]
-  rw [<-item_at_nat_to_fin' (h := ix₂.2)]
-  apply MerkleTree.item_at_nat_invariant (neq := fun h => neq (Fin.eq_of_veq h))
-
-lemma MerkleTree.item_at_fin_set_at_fin {H : Hash α 2} {tree : MerkleTree α H depth} {item: α} {ix: Fin (2 ^ depth)}:
-  tree_item_at_fin (tree.tree_set_at_fin ix item) ix = item := read_after_insert_sound _ _ _
 
 theorem ZMod.val_fin {n : ℕ } {f : ZMod n.succ}: f.val = Fin.val f := by
   simp [val]
@@ -108,48 +21,48 @@ theorem ZMod.val_fin {n : ℕ } {f : ZMod n.succ}: f.val = Fin.val f := by
 
 -- Insertion round semantic equivalence
 
-def insertion_round (Path: Vector F D) (Item: F) (PrevRoot: F) (Proof: Vector F D) (k: F -> Prop) : Prop :=
-  (MerkleTree.recover_tail poseidon₂ (Dir.create_dir_vec Path) Proof 0 = PrevRoot) ∧
-  k (MerkleTree.recover_tail poseidon₂ (Dir.create_dir_vec Path) Proof Item)
+-- def insertion_round (Path: Vector F D) (Item: F) (PrevRoot: F) (Proof: Vector F D) (k: F -> Prop) : Prop :=
+--   (MerkleTree.recover_tail poseidon₂ (Dir.create_dir_vec Path) Proof 0 = PrevRoot) ∧
+--   k (MerkleTree.recover_tail poseidon₂ (Dir.create_dir_vec Path) Proof Item)
 
-def insertion_round_prep (Index: F) (Item: F) (PrevRoot: F) (Proof: Vector F D) (k: F -> Prop) : Prop :=
-  ∃out: Vector F D, recover_binary_zmod' out = Index ∧ is_vector_binary out ∧
-  insertion_round out Item PrevRoot Proof k
+-- def insertion_round_prep (Index: F) (Item: F) (PrevRoot: F) (Proof: Vector F D) (k: F -> Prop) : Prop :=
+--   ∃out: Vector F D, recover_binary_zmod' out = Index ∧ is_vector_binary out ∧
+--   insertion_round out Item PrevRoot Proof k
 
-def fin_to_path (index : Nat) (d : Nat): Validate (index < 2^d) ⊕ Vector Dir d :=
-  if h : index < 2 ^ d then
-    Sum.inr (Dir.fin_to_dir_vec ⟨index, h⟩).reverse
-  else
-    Sum.inl ⟨h⟩
+-- def fin_to_path (index : Nat) (d : Nat): Validate (index < 2^d) ⊕ Vector Dir d :=
+--   if h : index < 2 ^ d then
+--     Sum.inr (Dir.fin_to_dir_vec ⟨index, h⟩).reverse
+--   else
+--     Sum.inl ⟨h⟩
 
-def tree_proof_at_validate (tree : MerkleTree α H d) (index : Nat): Validate (index < 2 ^ d) ⊕ Vector α d := do
-  let p ← fin_to_path index d
-  pure $ tree.proof p
+-- def tree_proof_at_validate (tree : MerkleTree α H d) (index : Nat): Validate (index < 2 ^ d) ⊕ Vector α d := do
+--   let p ← fin_to_path index d
+--   pure $ tree.proof p
 
-def insertionRound_semantics (Index Item : F) (Tree : MerkleTree F poseidon₂ D) (Proof : Vector F D) (k : MerkleTree F poseidon₂ D → Prop): Prop :=
+def insertionRoundSemantics (Index Item : F) (Tree : MerkleTree F poseidon₂ D) (Proof : Vector F D) (k : MerkleTree F poseidon₂ D → Prop): Prop :=
   if h : Index.val < 2 ^ D then
-    Tree.tree_item_at_fin ⟨Index.val, h⟩ = 0 ∧
-    Tree.tree_proof_at_fin ⟨Index.val, h⟩ = Proof.reverse ∧
-    k (Tree.tree_set_at_fin ⟨Index.val, h⟩ Item)
+    Tree.itemAtFin ⟨Index.val, h⟩ = 0 ∧
+    Tree.proofAtFin ⟨Index.val, h⟩ = Proof.reverse ∧
+    k (Tree.setAtFin ⟨Index.val, h⟩ Item)
   else False
 
 lemma Fin.castNat_lt_pow {n k : ℕ} (h : n < 2^k) : ↑n = Fin.mk n h := by
   apply Fin.eq_of_veq
   exact Nat.mod_eq_of_lt h
 
-theorem insertionRound_rw [Fact (CollisionResistant poseidon₂)] {Tree : MerkleTree F poseidon₂ D} :
+theorem insertionRoundCircuit_eq_insertionRoundSemantics [Fact (CollisionResistant poseidon₂)] {Tree : MerkleTree F poseidon₂ D} :
   gInsertionRound Index Item Tree.root Proof k ↔
-  insertionRound_semantics Index Item Tree Proof (fun t => k t.root) := by
-  simp [insertionRound_semantics, gInsertionRound]
+  insertionRoundSemantics Index Item Tree Proof (fun t => k t.root) := by
+  simp [insertionRoundSemantics, gInsertionRound]
   simp [Gates.to_binary, Gates.eq]
   simp [VerifyProof_looped, proof_rounds_uncps]
   apply Iff.intro
   . intro ⟨path, ⟨path_rec, path_bin⟩, _, hpre, _, hpost⟩
     split
     . rename_i h
-      unfold MerkleTree.tree_item_at_fin
-      unfold MerkleTree.tree_set_at_fin
-      unfold MerkleTree.tree_proof_at_fin
+      unfold MerkleTree.itemAtFin
+      unfold MerkleTree.setAtFin
+      unfold MerkleTree.proofAtFin
       simp_rw [←Fin.castNat_lt_pow h, Dir.recover_binary_zmod'_to_dir h (by decide) path_bin path_rec]
       have : MerkleTree.recover poseidon₂ (Dir.create_dir_vec path).reverse Proof.reverse 0 = Tree.root := by
         rw [←MerkleTree.recover_tail_equals_recover_reverse, ←hpre, ←Vector.ofFn_get (v := Proof)]
@@ -180,9 +93,9 @@ theorem insertionRound_rw [Fact (CollisionResistant poseidon₂)] {Tree : Merkle
       , fin_to_bits_recover_binary _ _
       , true_and
       ]
-    unfold MerkleTree.tree_item_at_fin at hitem
-    unfold MerkleTree.tree_set_at_fin at hnext
-    unfold MerkleTree.tree_proof_at_fin at hproof
+    unfold MerkleTree.itemAtFin at hitem
+    unfold MerkleTree.setAtFin at hnext
+    unfold MerkleTree.proofAtFin at hproof
     simp_rw [←Fin.castNat_lt_pow h] at hitem hnext hproof
     refine ⟨?_, ?_⟩
     . rw [MerkleTree.recover_tail_equals_recover_reverse]
@@ -203,7 +116,7 @@ def insertionRoundsSemantics {b : Nat}
   (proofs : Vector (Vector F D) b)
   (k : F → Prop): Prop := match b with
   | 0 => k tree.root
-  | Nat.succ _ => insertionRound_semantics
+  | Nat.succ _ => insertionRoundSemantics
       startIndex
       identities.head
       tree
@@ -218,17 +131,17 @@ theorem exists_binder {f : α → Prop} : (∃x, x = y ∧ f x) ↔ f y := by
   . intro hfy
     refine ⟨y, ⟨rfl, hfy⟩⟩
 
-theorem insertionRounds_rw [Fact (CollisionResistant poseidon₂)]  {Tree : MerkleTree F poseidon₂ D}:
+theorem insertionRoundsCircuit_eq_insertionRoundsSemantics [Fact (CollisionResistant poseidon₂)]  {Tree : MerkleTree F poseidon₂ D}:
   gInsertionProof startIndex Tree.root idComms merkleProofs k ↔
   insertionRoundsSemantics startIndex Tree idComms merkleProofs k := by
   unfold gInsertionProof
-  simp_rw [insertionRound_rw, Gates.add, exists_binder]
+  simp_rw [insertionRoundCircuit_eq_insertionRoundSemantics, Gates.add, exists_binder]
   apply Iff.of_eq
   simp only [add_zero]
 
   repeat (
     unfold insertionRoundsSemantics
-    cases idComms using Vector.casesOn; rename_i idComm idComms -- with | cons idComm idComms =>
+    cases idComms using Vector.casesOn; rename_i idComm idComms
     cases merkleProofs using Vector.casesOn; rename_i merkleProof merkleProofs
     try rw [add_assoc]
     congr
@@ -242,102 +155,99 @@ theorem insertionRounds_rw [Fact (CollisionResistant poseidon₂)]  {Tree : Merk
   try rw [add_assoc]
   congr
 
-def rootTransformationSpec'' {B : ℕ}
+def treeTransformationSemantics {B : ℕ}
   (tree : MerkleTree F poseidon₂ D)
   (identities : Vector F B)
   (startIndex : Nat): Option (MerkleTree F poseidon₂ D) := match B with
   | 0 => some tree
-  | _ + 1 => match tree.set_at_nat startIndex identities.head with
-    | some nextTree => rootTransformationSpec'' nextTree identities.tail (startIndex + 1)
-    | none => none
+  | _ + 1 => if h : startIndex < 2 ^ D
+    then treeTransformationSemantics (tree.setAtFin ⟨startIndex, h⟩ identities.head) identities.tail (startIndex + 1)
+    else none
 
-lemma rootTransformSpec_some_ix_bound {B : ℕ} {identities : Vector F B.succ}:
-  rootTransformationSpec'' tree identities startIndex = some tree' →
+lemma treeTransformationSemantics_some_index_bound {B : ℕ} {identities : Vector F B.succ}:
+  treeTransformationSemantics tree identities startIndex = some tree' →
   startIndex < 2 ^ D := by
   intro hp
-  conv at hp => lhs; whnf
+  unfold treeTransformationSemantics at hp
   split at hp
-  . apply MerkleTree.set_at_nat_some_when_le
-    assumption
+  . assumption
   . contradiction
 
-lemma rootTransformSpec_succ {B : ℕ} {identities : Vector F B.succ}
-  (hp : rootTransformationSpec'' tree identities startIndex = some tree'):
-  rootTransformationSpec''
-    (tree.tree_set_at_fin ⟨startIndex, rootTransformSpec_some_ix_bound hp⟩ identities.head)
+lemma treeTransformationSemantics_next {B : ℕ} {identities : Vector F B.succ}
+  (hp : treeTransformationSemantics tree identities startIndex = some tree'):
+  treeTransformationSemantics
+    (tree.setAtFin ⟨startIndex, treeTransformationSemantics_some_index_bound hp⟩ identities.head)
     identities.tail
     (startIndex + 1) = some tree' := by
-    have bound : startIndex < 2 ^ D := rootTransformSpec_some_ix_bound hp
-    conv at hp => lhs; whnf
+    have bound : startIndex < 2 ^ D := treeTransformationSemantics_some_index_bound hp
+    unfold treeTransformationSemantics at hp
     split at hp
     . rename_i h
-      rw [MerkleTree.set_at_nat_to_fin' (h:=bound)] at h
-      injection h with h
-      rwa [h]
+      assumption
     . contradiction
+
+-- theorem insertionRoundsRootTransformation
+--   {B : ℕ} {startIndex : Nat} {identities : Vector F B} {proofs : Vector (Vector F D) B}
+--   (indexIsValid : startIndex + B < 2 ^ D):
+--   insertionRoundsSemantics startIndex tree identities proofs k →
+--   ∃postTree, treeTransformationSemantics tree identities startIndex = some postTree ∧ k postTree.root := by
+--   intro hp
+--   induction B generalizing startIndex tree with
+--   | zero => exists tree
+--   | succ B ih =>
+--     unfold insertionRoundsSemantics at hp
+--     unfold insertionRoundSemantics at hp
+--     split at hp
+--     . rename_i bound
+--       rcases hp with ⟨-, -, hp⟩
+--       have := by
+--         refine ih ?_ hp
+--         rw [add_assoc]
+--         apply Nat.lt_of_le_of_lt
+--         . apply Nat.add_le_add_right
+--           apply Nat.mod_le
+--         . simp; linarith
+--       have ixLeOrd : startIndex < Order := by
+--         apply LT.lt.trans
+--         apply Nat.lt_sub_of_add_lt
+--         exact indexIsValid
+--         apply Nat.lt_of_le_of_lt
+--         apply Nat.sub_le
+--         decide
+--       rcases this with ⟨t, hsome, hk⟩
+--       exists t
+--       unfold treeTransformationSemantics
+--       apply And.intro
+--       . rw [←hsome]
+--         split
+--         . congr
+--           . exact Eq.symm (ZMod.val_cast_of_lt ixLeOrd)
+--           . exact Eq.symm (Nat.mod_eq_of_lt ixLeOrd)
+--         . rename_i h
+--           exfalso
+--           apply h
+--           linarith
+--       . exact hk
+--     . contradiction
 
 theorem insertionRoundsRootTransformation
-  {B : ℕ} {startIndex : Nat} {identities : Vector F B} {proofs : Vector (Vector F D) B}
-  (indexIsValid : startIndex + B < 2 ^ D):
-  insertionRoundsSemantics startIndex tree identities proofs k →
-  ∃postTree, rootTransformationSpec'' tree identities startIndex = some postTree ∧ k postTree.root := by
-  intro hp
-  induction B generalizing startIndex tree with
-  | zero => exists tree
-  | succ B ih =>
-    unfold insertionRoundsSemantics at hp
-    unfold insertionRound_semantics at hp
-    split at hp
-    . rename_i bound
-      rcases hp with ⟨-, -, hp⟩
-      have := by
-        refine ih ?_ hp
-        rw [add_assoc]
-        apply Nat.lt_of_le_of_lt
-        . apply Nat.add_le_add_right
-          apply Nat.mod_le
-        . simp; linarith
-      have ixLeOrd : startIndex < Order := by
-        apply LT.lt.trans
-        apply Nat.lt_sub_of_add_lt
-        exact indexIsValid
-        apply Nat.lt_of_le_of_lt
-        apply Nat.sub_le
-        decide
-      rcases this with ⟨t, hsome, hk⟩
-      exists t
-      conv => arg 1; lhs; whnf
-      rw [MerkleTree.set_at_nat_to_fin']
-      simp
-      apply And.intro
-      . rw [←hsome]
-        congr
-        . exact Eq.symm (ZMod.val_cast_of_lt ixLeOrd)
-        . exact Eq.symm (Nat.mod_eq_of_lt ixLeOrd)
-        . rw [ZMod.val_cast_of_lt ixLeOrd] at bound; exact bound
-      . exact hk
-    . contradiction
-
-theorem insertionRoundsRootTransformation'
   {B : ℕ} {startIndex : F} {identities : Vector F B} {proofs : Vector (Vector F D) B}:
-  -- (indexIsValid : startIndex + B < 2 ^ D):
   insertionRoundsSemantics startIndex tree identities proofs k →
-  ∃postTree, rootTransformationSpec'' tree identities startIndex.val = some postTree ∧ k postTree.root := by
+  ∃postTree, treeTransformationSemantics tree identities startIndex.val = some postTree ∧ k postTree.root := by
   intro hp
   induction B generalizing startIndex tree with
   | zero => exists tree
   | succ B ih =>
     unfold insertionRoundsSemantics at hp
-    unfold insertionRound_semantics at hp
+    unfold insertionRoundSemantics at hp
     split at hp
     . rename_i bound
       rcases hp with ⟨-, -, hp⟩
       have := ih hp
       rcases this with ⟨t, hsome, hk⟩
       exists t
-      conv => arg 1; lhs; whnf
-      rw [MerkleTree.set_at_nat_to_fin']
-      simp
+      unfold treeTransformationSemantics
+      split; rotate_left; exfalso; rename_i h; exact h bound
       apply And.intro
       . rw [←hsome]
         congr
@@ -353,7 +263,7 @@ theorem insertionRoundsRootTransformation'
 theorem before_insertion_all_zero
   {B: ℕ} {startIndex : F} {proofs : Vector (Vector F D) B} {identities : Vector F B}:
   insertionRoundsSemantics (b := B) startIndex tree identities proofs k →
-  ∀i ∈ [startIndex.val : (startIndex + B).val], tree.item_at_nat i = some 0 := by
+  ∀i ∈ [startIndex.val : (startIndex + B).val], tree[i]? = some 0 := by
   intro hp i hi
 
   induction B generalizing i startIndex tree with
@@ -368,13 +278,15 @@ theorem before_insertion_all_zero
     cases identities using Vector.casesOn with | cons id ids =>
     cases proofs using Vector.casesOn with | cons proof proofs =>
     unfold insertionRoundsSemantics at hp
-    unfold insertionRound_semantics at hp
+    unfold insertionRoundSemantics at hp
     rcases hi with ⟨hil, hiu⟩
     split at hp
     . cases hil
       . rcases hp with ⟨hp, -, -⟩
         rename_i h
-        rw [MerkleTree.item_at_nat_to_fin', hp]
+        rw [getElem?_eq_some_getElem_of_valid_index]
+        . simp [getElem, hp]
+        . exact h
       . rename_i i hil
         rcases hp with ⟨-, -, hp⟩
         have := ih hp (i.succ) (by
@@ -389,13 +301,11 @@ theorem before_insertion_all_zero
             simp [add_assoc]
             rw [add_comm (b:=1)]
         )
-        have bound := MerkleTree.item_at_nat_some_when_le this
-        rw [MerkleTree.item_at_nat_to_fin' _ _ bound] at this
-        rw [MerkleTree.item_at_fin_invariant'] at this
-        rw [←MerkleTree.item_at_nat_to_fin' _ _ bound] at this
-        assumption
-        rfl
+        have := getElem_of_getElem?_some this
+        rw [MerkleTree.getElem_setAtFin_invariant_of_neq] at this
+        exact getElem?_some_of_getElem this
         simp
+        rw [eq_comm]
         apply Nat.ne_of_lt
         apply Nat.lt_succ_of_le
         assumption
@@ -408,14 +318,14 @@ theorem ix_bound {B : ℕ} {startIndex : F} {identities : Vector F B.succ} {proo
   | zero =>
     intro hp
     unfold insertionRoundsSemantics at hp
-    unfold insertionRound_semantics at hp
+    unfold insertionRoundSemantics at hp
     split at hp
     . simpa
     . contradiction
   | succ B ih =>
     intro hp
     unfold insertionRoundsSemantics at hp
-    unfold insertionRound_semantics at hp
+    unfold insertionRoundSemantics at hp
     split at hp
     . rename_i hi
       rcases hp with ⟨-, -, hp⟩
@@ -430,13 +340,10 @@ theorem ix_bound {B : ℕ} {startIndex : F} {identities : Vector F B.succ} {proo
         exact LT.lt.trans hi (by decide)
     . contradiction
 
-instance : Decidable (i ∈ [a : b]) := by
-  simp [Membership.mem]; infer_instance
-
 lemma treeTransform_get_lt {i : Nat} {B : ℕ} {startIndex : Nat}
   {identities : Vector F B}:
-  rootTransformationSpec'' tree identities startIndex = some tree' →
-  i < startIndex → tree.item_at_nat i = tree'.item_at_nat i := by
+  treeTransformationSemantics tree identities startIndex = some tree' →
+  i < startIndex → tree[i]? = tree'[i]? := by
   induction B generalizing startIndex tree tree' with
   | zero =>
     intro h _
@@ -446,28 +353,23 @@ lemma treeTransform_get_lt {i : Nat} {B : ℕ} {startIndex : Nat}
   | succ B ih =>
     intro h hu
     cases identities using Vector.casesOn
-    conv at h => lhs; whnf
+    unfold treeTransformationSemantics at h
     split at h
     . rename_i hp'
       have := ih h (by linarith)
       rw [←this]
-      have sibound : startIndex < 2^D := MerkleTree.set_at_nat_some_when_le hp'
-      have ibound : i < 2^D := lt_trans hu sibound
-      rw [MerkleTree.set_at_nat_to_fin_some' (h:=sibound)] at hp'
-      rw [MerkleTree.item_at_nat_to_fin' (h:=ibound)]
-      rw [MerkleTree.item_at_nat_to_fin' (h:=ibound)]
+      have ibound : i < 2^D := lt_trans hu hp'
+      repeat rw [getElem?_eq_some_getElem_of_valid_index (cont := MerkleTree _ _ _) ibound]
       apply congrArg
-      apply Eq.symm
-      apply MerkleTree.item_at_fin_invariant' hp'
-      intro hp
-      injection hp with hp
-      exact Nat.ne_of_lt hu (eq_comm.mp hp)
+      rw [eq_comm]
+      apply MerkleTree.getElem_setAtFin_invariant_of_neq
+      apply Nat.ne_of_lt hu
     . contradiction
 
 lemma treeTransform_get_gt {i B startIndex : ℕ}
   {identities : Vector F B}:
-  rootTransformationSpec'' tree identities startIndex = some tree' →
-  i ≥ startIndex + B → tree.item_at_nat i = tree'.item_at_nat i := by
+  treeTransformationSemantics tree identities startIndex = some tree' →
+  i ≥ startIndex + B → tree[i]? = tree'[i]? := by
   induction B generalizing startIndex tree tree' with
   | zero =>
     intro h _
@@ -477,43 +379,40 @@ lemma treeTransform_get_gt {i B startIndex : ℕ}
   | succ B ih =>
     intro h hl
     cases identities using Vector.casesOn
-    conv at h => lhs; whnf
+    unfold treeTransformationSemantics at h
     split at h
     . cases Nat.lt_or_ge i (2^D) with
       | inl ibound =>
-        rename_i hp
-        have sibound : startIndex < 2^D := MerkleTree.set_at_nat_some_when_le hp
-        repeat rw [MerkleTree.item_at_nat_to_fin' (h:=ibound)]
-        rw [MerkleTree.set_at_nat_to_fin_some' (h:=sibound)] at hp
+        rename_i sibound
         have := ih h (by linarith)
-        repeat rw [MerkleTree.item_at_nat_to_fin' (h:=ibound)] at this
-        rw [←this]
+        rw [←ih h (by linarith)]
+        repeat rw [getElem?_eq_some_getElem_of_valid_index (cont := MerkleTree _ _ _) ibound]
         apply congrArg
-        apply Eq.symm
-        apply MerkleTree.item_at_fin_invariant' hp
-        intro hp
-        injection hp with hp
+        rw [eq_comm]
+        apply MerkleTree.getElem_setAtFin_invariant_of_neq
         linarith
       | inr h =>
-        simp_rw [MerkleTree.item_at_nat_none_when_ge h]
+        repeat rw [getElem?_none_of_invalid_index]
+        all_goals exact not_lt_of_ge h
     . contradiction
 
 lemma treeTransform_get_inrange {i B startIndex : ℕ} {identities : Vector F B}
-  (hp : rootTransformationSpec'' tree identities startIndex = some tree')
+  (hp : treeTransformationSemantics tree identities startIndex = some tree')
   (inrange : i ∈ [0 : B]):
-  tree'.item_at_nat (startIndex + i) = identities[i]'inrange.2 := by
+  tree'[startIndex + i]? = identities[i]'inrange.2 := by
   induction B generalizing startIndex i tree tree' with
   | zero => cases inrange; exfalso; linarith
   | succ B ih =>
-    have := rootTransformSpec_succ hp
-    have bound := rootTransformSpec_some_ix_bound hp
+    have := treeTransformationSemantics_next hp
+    have bound := treeTransformationSemantics_some_index_bound hp
     cases identities using Vector.casesOn with | cons id ids =>
     cases i with
     | zero =>
       have := treeTransform_get_lt this (by linarith)
+      rw [getElem?_eq_some_getElem_of_valid_index (cont := MerkleTree _ _ _) bound] at this
       simp
-      rw [←this, MerkleTree.item_at_nat_to_fin_some' _ _ bound]
-      simp
+      rw [←this]
+      apply congrArg
       apply MerkleTree.read_after_insert_sound
     | succ i =>
       have inrange : i ∈ [0 : B] := by
@@ -523,5 +422,4 @@ lemma treeTransform_get_inrange {i B startIndex : ℕ} {identities : Vector F B}
       simp
       simp at this
       rw [←this]
-      apply congrArg
-      simp_arith
+      rw [Nat.succ_eq_one_add, add_assoc]
